stv as list and aes evaluation

xc/network_semantics.v
@@ -4,6 +4,7 @@ From AC Require Import sensor_state.
 From AC Require Import value_tree.
 From AC Require Import nvalues.
 From AC Require Import big_step_semantics.
+From AC Require Import tactics.
 Require Import Bool.
 Require Import String.
 Require Import List.
@@ -55,6 +56,8 @@ Definition add_s (new_e:event) (new_s:sensor_state) (old:s_net): s_net :=(fun e 
 (*The augmented event structure, like defined in the papers*)
 Inductive AES := aes : E_net -> R_net -> d_net -> s_net -> AES.
 
+
+(* Old function formalisation
 (*Space time values, a function that maps each event to a resulting nvalue*)
 Definition STV := event -> nvalue.
 Definition base_STV (e:event) := default l_fail.
@@ -64,15 +67,135 @@ Definition add_STV (new_e:event) (new_w:nvalue) (old:STV): STV := (fun e => if (
 Definition vt_net := event -> value_tree.
 Definition base_vt (e:event) := empty nil.
 Definition add_vt (new_e:event) (new_vt:value_tree) (old:vt_net): vt_net :=(fun e => if (equalsEv e new_e) then new_vt else (old e)).
+*) 
+ 
 
-(*A function that return the source events of a event*)
-Fixpoint before_event (b_e:event) (b_E:E_net) (b_R:R_net) (b_vts:vt_net) (b_d:d_net): value_tree_env :=
-match b_E with 
-| cons e_el next => if (containsR (forward e_el b_e) b_R) then vt_el (b_d e_el) (b_vts e_el) (before_event b_e next b_R b_vts b_d) 
-else (before_event b_e next b_R b_vts b_d)
-| nil => vt_end
+Inductive STV_el := net_w_el : event -> nvalue -> STV_el. 
+Definition STV := list STV_el.
+Inductive vt_net_el := net_vt_el : event -> value_tree -> vt_net_el. 
+Definition vt_net := list vt_net_el. 
+
+
+
+
+Fixpoint before_event (b_e:event) (b_E:E_net) (b_R:R_net) (b_vts:vt_net) (b_d:d_net): value_tree_env := 
+match (b_E,b_vts) with 
+| (cons el0 next,cons (net_vt_el el1 vt) next_vt) => if ((containsR (forward el0 b_e) b_R) && (equalsEv el0 el1) ) then vt_el (b_d el0) (vt) (before_event b_e next b_R next_vt b_d) 
+else (before_event b_e next b_R next_vt b_d)
+| (nil,nil) => vt_end
+| _ => vt_end
 end.
 
+Definition notNone {A:Type} (op:option A) :=
+match op with
+| Some _ => true
+| None => false
+end.
+
+
+(*With optional result variant of before_event*)
+Definition add_vts_el (d:nat) (vt:value_tree) (vts:value_tree_env) := vt_el d vt vts. 
+Fixpoint before_event_option (b_e:event) (b_E:E_net) (b_R:R_net) (b_vts:vt_net) (b_d:d_net): option value_tree_env := 
+match (b_E,b_vts) with 
+| (cons el0 next,cons (net_vt_el el1 vt) next_vt) => 
+  if (equalsEv el0 el1) then 
+      (let x:=before_event_option b_e next b_R next_vt b_d in 
+      if (containsR (forward el0 b_e) b_R) then (option_map (add_vts_el (b_d el0) vt) x) else (x)
+      )
+  else None
+| (nil,nil) => Some vt_end
+| _ => None
+end. 
+
+Inductive net_conf_in: Type := netI : AES -> exp -> net_conf_in.
+Inductive net_conf_out: Type := netO : STV -> vt_net -> net_conf_out.
+
+Reserved Notation "t '|=>' t'" (at level 40).
+Inductive net_val: net_conf_in -> net_conf_out -> Prop :=
+
+| E_NET_0 : forall (e_main:exp) (n_R:R_net) (n_d:d_net) (n_s:s_net),
+
+netI (aes (nil) n_R n_d n_s) e_main |=> netO nil nil
+
+
+| E_NET_R : forall (e_main:exp) (ev:event) (next:E_net) (n_R:R_net) (n_d:d_net) (n_s:s_net) (w:nvalue) 
+(next_stv:STV) (vt:value_tree) (next_vts:vt_net) (vt_env:value_tree_env),
+
+netI (aes next n_R n_d n_s) e_main |=> netO next_stv next_vts
+
+Some vt_env = before_event_option ev next n_R next_vts n_d  
+
+-> <[ n_d ev | n_s ev | (before_event ev next n_R next_vts n_d) | e_main ]> ==> <[ w |  vt ]> 
+
+-> netI (aes (cons ev next) n_R n_d n_s) e_main |=> netO (cons (net_w_el ev w) next_stv)  (cons (net_vt_el ev vt) next_vts) 
+
+where "t '|=>' t'" := (net_val t t').
+
+
+
+
+
+
+(*
+
+Definition fun_ex: string := "fun0". 
+Definition fun_or_x: string := "fun_or_x". 
+Definition fun_or_y: string := "fun_or_y". 
+Definition f1: string := "f1". 
+Definition f2: string := "f2". 
+Definition old: string := "old". 
+Definition x: string := "x". 
+Definition y: string := "y". 
+
+Definition eventList: E_net := (e 0 2) :: (e 1 2) :: (e 2 2) :: (e 0 1) :: (e 1 1) :: (e 2 1) ::  (e 0 0) :: (e 1 0) :: (e 2 0) :: nil.
+
+Definition messageList: R_net := forward (e 0 1) (e 0 2) :: forward (e 0 1) (e 2 2) ::
+forward (e 1 1) (e 0 2) :: forward (e 1 1) (e 1 2) :: forward (e 1 1) (e 2 2) :: forward (e 2 1) (e 0 2) :: 
+forward (e 2 1) (e 2 2) :: forward (e 0 0) (e 0 1) :: forward (e 0 0) (e 1 1) :: forward (e 1 0) (e 1 1) ::
+forward (e 2 0) (e 1 1) :: forward (e 2 0) (e 2 1) :: nil.
+
+Definition deviceMap (e:event): nat :=  match e with | (e id n) => id end.
+
+Definition sensorMap (ev:event): sensor_state := add f1 <{[>false]}> (add f2 <{[>true]}> base).
+
+(*
+match ev with 
+| e 0 0 => add f1 <{[>false]}> (add f2 <{[>true]}> base)
+| e 0 1 => add f1 <{[>true]}> (add f2 <{[>false]}> base)
+| e 0 2 => add f1 <{[>false]}> (add f2 <{[>true]}> base)
+| e 1 1 => add f1 <{[>true]}> (add f2 <{[>false]}> base)
+| e 1 _ => add f1 <{[>false]}> (add f2 <{[>false]}> base)
+| e _ _ => add f1 <{[>true]}> (add f2 <{[>false]}> base)
+end.
+*)
+
+Definition exp_main: exp := 
+<{app exchange $(false) (fun fun_ex[old] {app b_or $(sensor f2) (app b_and $(sensor f1) (app nfold $ (fun fun_or_x[x] {fun fun_or_y[y] {app b_or $x y$} }) (old) (false)$)$ )$ }) $ }> .
+
+
+Lemma one_lemma : exists (stv:STV) (vts:vt_net), 
+netI (aes eventList messageList deviceMap sensorMap) <{exp_main}> |=> netO stv vts .
+Proof.
+eexists. eexists.
+repeat eapply E_NET_R. eapply E_NET_0.
+1-2:[>auto|device_tac].
+1-2:[>auto|device_tac].
+1-2:[>auto|device_tac].
+1-2:[>auto|device_tac].
+1-2:[>auto|device_tac].
+1-2:[>auto|device_tac].
+1-2:[>auto|device_tac].
+1-2:[>auto|device_tac].
+1-2:[>auto|device_tac].
+Qed.
+
+*)
+
+
+
+
+
+(*
 
 (*Function that check if a event is sourced by another event in a list*)
 Fixpoint isSourcedBy (ev:event) (evList:E_net) (is_R:R_net) : bool :=
@@ -88,7 +211,6 @@ match rts_rec_E with
 | cons (ev) next => if (isSourcedBy ev rts_all_E rts_R) then returnNotSourced next rts_all_E rts_R else Some ev
 | nil => None
 end.
-
 
 
 Fixpoint removeEv (ev:event) (evList:E_net) :=
@@ -122,7 +244,7 @@ netI (aes n_E n_R n_d n_s) ev_notExplored vt_collected e_main |=> n_stv
 
 where "t '|=>' t'" := (net_val t t').
 
-
+*)
 
 (*
 Inductive net_conf_in: Type := netI : AES -> exp -> net_conf_in.
